more refactoring to unify Abstract Machines used for Turing machines with the ones used in L

theories/L/AbstractMachines/Programs.v
@@ -1,25 +1,8 @@
 From Undecidability.L Require Import Prelim.MoreBase L AbstractMachines.LargestVar.
 Require Import Lia.
+Require Export Undecidability.L.AbstractMachines.ProgramsDef.
 
 (** * Abstract L machines *)
-(** ** Encoding Terms as Programs *)
-
-Inductive Tok := varT (n :nat) | appT | lamT | retT.
-Notation Pro := (list Tok) (only parsing).
-
-Instance Tok_eq_dec : eq_dec Tok.
-repeat intro. hnf. repeat decide equality.
-Qed.
-
-Fixpoint compile (s: L.term) : Pro :=
-  match s with
-    var x => [varT x]
-  | app s t => compile s ++ compile t ++ [appT]
-  | lam s => lamT :: compile s ++ [retT]
-  end.
-
-Inductive reprP : Pro -> term -> Prop :=
-  reprPC s : reprP (compile s) (lam s).
 
 (** *** Program size *)
 
