theories/L/Complexity/Reductions/TMGenNP/IntermediateProblems.v
@@ -1,3 +1,4 @@
+From Undecidability.L Require Import Tactics.LTactics Prelim.MoreList Prelim.MoreBase.
 From Undecidability.L.Complexity Require Import NP Synthetic Monotonic GenNPHalt.
 
 
@@ -25,18 +26,44 @@ Check NPhard_GenNP.
 
 (** Have: Implementation of Heap-based machine (Not step-indexed) *)
 
-From Undecidability.LAM  Require TM.HaltingProblem.
+From Undecidability.LAM  Require LM_heap_def LM_heap_correct.
+From Undecidability.L Require AbstractMachines.Computable.Shared.
+Section LMGenNPHalt.
+  Import LM_heap_def LM_heap_correct.
+
+  Definition initLMGen s c : (list (nat*list Tok)*list (nat*list Tok)*list (option ((nat * list Tok) * nat))):= ([(0,s)],[(0,c)],[]).
+  Definition LMGenNPHalt' : list Tok*nat*nat -> Prop :=
+    fun '(s, maxSize, steps (*in unary*)) =>
+      exists (c:list Tok), size (enc c) <= maxSize /\ halts_k (initLMGen s c) steps.
+
+  Definition LMHaltsOrDiverges : list Tok*nat*nat -> Prop :=
+    fun '(s, maxSize, steps (*in unary*)) =>
+      exists c, size (enc c) <= maxSize -> forall k, halts_k (initLMGen s c) k -> k <= steps.
+
+  Definition LMGenNPHalt := restrictBy LMHaltsOrDiverges LMGenNPHalt'.
+
+  Lemma polyRed_GenNPHalt_to_LMGenNPHalt :
+    GenNPHalt ⪯p LMGenNPHalt.
+  Proof.
+    pose (f := (fun '(s, maxSize, steps) => ([appT],cnst 0,cnst 1)): (term * nat * nat) -> _);cbn beta in f.
+    eapply reducesPolyMO_intro with (f:=f).
 
 
-Print HaltingProblem.Loop_Rel.
-Print HaltingProblem.Loop_T.
+  
+
+  From Undecidability.LAM  Require TM.HaltingProblem.
+  About HaltingProblem.Loop_Rel.
+  About HaltingProblem.Loop_T.
+
+  Abort.
+End LMGenNPHalt.
+
 
 (** Not Complete: nice form of Time bound *)
 From Undecidability.LAM  Require TM.LMBounds.
-Print LMBounds.LM.
 
 
 (** Approach: simulate step-indexed L interpreter inside TM *)
 (** Problems: Well-formedness of certificate-input? *)
 
-(** Maybe intermediate problem in terms of Heap-Machine?)
+(** Maybe intermediate problem in terms of Heap-Machine? *)
