theories/LAM/TM/CaseCom.v
@@ -10,7 +10,7 @@ Definition CaseCom : pTM sigCom^+ (option ACom) 1 :=
      (Relabel (ChangeAlphabet (CaseFin (FinType(EqType(ACom))) ) _) Some).
 
 
-Definition CaseCom_size (t : Com) : nat -> nat :=
+Definition CaseCom_size (t : Tok) : nat -> nat :=
   match t with
   | varT n => S
   | _ => S >> S >> S
@@ -18,7 +18,7 @@ Definition CaseCom_size (t : Com) : nat -> nat :=
 
 Definition CaseCom_Rel : pRel sigCom^+ (FinType (EqType (option ACom))) 1 :=
   fun tin '(yout, tout) =>
-    forall (t : Com) (s : nat),
+    forall (t : Tok) (s : nat),
       tin[@Fin0] ≃(;s) t ->
       match yout, t with
       | Some appAT, appT => isRight_size tout[@Fin0] (CaseCom_size t s)
